BoogieLang/TypeSafety.thy
@@ -14,30 +14,30 @@ fun expr_is_defined :: "'a nstate \<Rightarrow> expr \<Rightarrow> bool"
    | "expr_is_defined ns (ForallT e) = expr_is_defined ns e"
    | "expr_is_defined ns (ExistsT e) = expr_is_defined ns e"
 
-lemma unop_type_correct: "\<lbrakk> unop_type uop = (arg_ty, ret_ty); type_of_val A v' = Some (TPrim arg_ty);
+lemma unop_type_correct: "\<lbrakk> unop_type uop = (arg_ty, ret_ty); type_of_val A v' = TPrim arg_ty;
                          (unop_eval_val uop v') = Some v  \<rbrakk> \<Longrightarrow>
-                       type_of_val A v = Some (TPrim ret_ty)"
+                       type_of_val A v = TPrim ret_ty"
   by (cases uop; rule lit_val_elim[where v=v']; auto)
 
-lemma unop_progress: "\<lbrakk> unop_type uop = (arg_ty, ret_ty); type_of_val A v' = Some (TPrim arg_ty) \<rbrakk> \<Longrightarrow>
+lemma unop_progress: "\<lbrakk> unop_type uop = (arg_ty, ret_ty); type_of_val A v' = TPrim arg_ty\<rbrakk> \<Longrightarrow>
                        \<exists>v. (unop_eval_val uop v') = Some v "
   by (cases uop; rule lit_val_elim[where v=v']; auto)
 
 lemma binop_type_correct: 
  "\<lbrakk> binop_type bop = Some ((left_ty,right_ty), ret_ty); 
-    type_of_val  A v1 = Some (TPrim left_ty); type_of_val A v2 = Some (TPrim right_ty); 
+    type_of_val  A v1 = (TPrim left_ty); type_of_val A v2 = (TPrim right_ty); 
     (binop_eval_val bop v1 v2) = Some v  \<rbrakk> \<Longrightarrow>
-    type_of_val A v = Some (TPrim ret_ty)"
+    type_of_val A v = TPrim ret_ty"
   by (cases bop; rule lit_val_elim[where v=v1]; rule lit_val_elim[where v=v2]; auto)
 
 lemma binop_progress:
  "\<lbrakk> binop_type bop = Some ((left_ty,right_ty), ret_ty); 
-    type_of_val  A v1 = Some (TPrim left_ty); type_of_val A v2 = Some (TPrim right_ty)\<rbrakk> \<Longrightarrow>
+    type_of_val  A v1 = TPrim left_ty; type_of_val A v2 = TPrim right_ty\<rbrakk> \<Longrightarrow>
     \<exists>v. (binop_eval_val bop v1 v2) = Some v "
   by (cases bop; rule lit_val_elim[where v=v1]; rule lit_val_elim[where v=v2]; auto)
 
 lemma binop_poly_type_correct:
- "\<lbrakk> binop_poly_type bop; binop_eval_val bop v1 v2 = Some v \<rbrakk> \<Longrightarrow> type_of_val A v = Some (TPrim TBool)"
+ "\<lbrakk> binop_poly_type bop; binop_eval_val bop v1 v2 = Some v \<rbrakk> \<Longrightarrow> type_of_val A v = TPrim TBool"
   by (cases bop; rule lit_val_elim[where v=v1]; rule lit_val_elim[where v=v2]; auto)
 
 text\<open>check whether the free variables of a type are at smaller than some value\<close>
@@ -137,12 +137,12 @@ lemma map_map:
 theorem preservation:
   assumes 
           "list_all closed \<Omega>"
-          "\<forall> k \<tau>'. (\<Delta> k = Some \<tau>') \<longrightarrow> (\<exists>v. (n_s k = Some v) \<and> type_of_val A v = Some (instantiate \<Omega> \<tau>'))" and
+          "\<forall> k \<tau>'. (\<Delta> k = Some \<tau>') \<longrightarrow> (\<exists>v. (n_s k = Some v) \<and> type_of_val A v = instantiate \<Omega> \<tau>')" and
           Wf_\<Gamma>:"fun_interp_wf A F \<Gamma>" and
           Wf_F:"list_all (wf_fdecl \<circ> snd) F" 
-  shows "F, \<Delta> \<turnstile> e : \<tau> \<Longrightarrow> wf_expr (length \<Omega>) e \<Longrightarrow> A,(F,\<Gamma>),\<Omega> \<turnstile> \<langle>e,n_s\<rangle> \<Down> v \<Longrightarrow> type_of_val A v = Some (instantiate \<Omega> \<tau>)" and 
+  shows "F, \<Delta> \<turnstile> e : \<tau> \<Longrightarrow> wf_expr (length \<Omega>) e \<Longrightarrow> A,(F,\<Gamma>),\<Omega> \<turnstile> \<langle>e,n_s\<rangle> \<Down> v \<Longrightarrow> type_of_val A v = instantiate \<Omega> \<tau>" and 
         "F, \<Delta> \<turnstile> es [:] ts \<Longrightarrow> list_all (wf_expr (length \<Omega>)) es \<Longrightarrow> A,(F,\<Gamma>),\<Omega> \<turnstile> \<langle>es,n_s\<rangle> [\<Down>] vs \<Longrightarrow>
-          map (type_of_val A) vs = map Some (map (instantiate \<Omega>) ts)"
+          map (type_of_val A) vs = (map (instantiate \<Omega>) ts)"
   using assms
 proof (induction arbitrary: v \<Omega> and vs \<Omega> rule: typing_typing_list.inducts)
   case (TypVar \<Delta> x ty)
@@ -154,7 +154,7 @@ next
   case (TypUnOp uop arg_ty ret_ty \<Delta> e)
   from this obtain v' where 
      "A,(F, \<Gamma>),\<Omega> \<turnstile> \<langle>e,n_s\<rangle> \<Down> v'" and "unop_eval_val uop v' = Some v" by auto
-  moreover from this have "type_of_val A v' = Some (TPrim arg_ty)" using TypUnOp by auto
+  moreover from this have "type_of_val A v' = TPrim arg_ty" using TypUnOp by auto
   ultimately show ?case using \<open>unop_type uop = (arg_ty, ret_ty)\<close> unop_type_correct by fastforce 
 next
   case (TypBinOpMono bop left_ty right_ty ret_ty \<Delta> e1 e2)
@@ -162,8 +162,8 @@ next
      "A, (F, \<Gamma>),\<Omega> \<turnstile> \<langle>e1, n_s\<rangle> \<Down> v1" and "A, (F, \<Gamma>), \<Omega> \<turnstile> \<langle>e2, n_s\<rangle> \<Down> v2" and 
      E:"binop_eval_val bop v1 v2 = Some v"
     by auto
-  moreover from this have T1:"type_of_val A v1 = Some (TPrim left_ty)" and 
-    T2:"type_of_val A v2 = Some (TPrim right_ty)" using TypBinOpMono by auto
+  moreover from this have T1:"type_of_val A v1 = TPrim left_ty" and 
+    T2:"type_of_val A v2 = TPrim right_ty" using TypBinOpMono by auto
   ultimately show ?case using \<open>binop_type bop = Some ((left_ty, right_ty), ret_ty)\<close> binop_type_correct by fastforce
 next
   case (TypBinopPoly bop \<Delta> e1 ty1 e2 ty2 ty_inst)
@@ -197,9 +197,9 @@ next
     apply (rule instantiate_msubst_opt)
     by (simp add: list.pred_set)   
   have
-   "map (type_of_val A) vargs = map Some (map (instantiate \<Omega>) (map (msubstT_opt ty_params) args_ty))"
+   "map (type_of_val A) vargs = (map (instantiate \<Omega>) (map (msubstT_opt ty_params) args_ty))"
     using TypFunExp.IH RedArgs TypFunExp.prems(3) TypFunExp.prems(4) TypFunExp.prems(5) TypFunExp.prems(6) \<open>list_all (wf_expr (length \<Omega>)) args\<close> by blast
-  hence "type_of_val A v = Some (instantiate (map (instantiate \<Omega>) ty_params) ret_ty)"
+  hence "type_of_val A v = instantiate (map (instantiate \<Omega>) ty_params) ret_ty"
     apply (simp only: InstMSubst)
     using FunSingleWf A1 A3 A4 
     apply auto
@@ -226,8 +226,8 @@ next
   from \<open>A,(F, \<Gamma>),\<Omega> \<turnstile> \<langle>(e # es),n_s\<rangle> [\<Down>] vs\<close> have
   "A,(F, \<Gamma>),\<Omega> \<turnstile> \<langle>e, n_s\<rangle> \<Down> hd vs" and "A,(F, \<Gamma>),\<Omega> \<turnstile> \<langle>es, n_s\<rangle> [\<Down>] tl vs" 
       using cons_exp_elim by auto
-  with TypListCons have A1:"type_of_val A (hd vs) = Some ((instantiate \<Omega>) ty)" and
-                        A2:"map (type_of_val A) (tl vs) = map Some (map (instantiate \<Omega>) tys)"
+  with TypListCons have A1:"type_of_val A (hd vs) = instantiate \<Omega> ty" and
+                        A2:"map (type_of_val A) (tl vs) = map (instantiate \<Omega>) tys"
     by auto
   moreover have "(hd vs) # (tl vs) = vs" using \<open>A,(F, \<Gamma>),\<Omega> \<turnstile> \<langle>(e # es),n_s\<rangle> [\<Down>] vs\<close> 
       using cons_exp_elim list.collapse by blast
@@ -244,12 +244,14 @@ lemma env_corres_extend:
   by simp  
 *)
 
+(*
 lemma
   assumes "\<forall>k \<tau>'.
            \<Delta> k = Some \<tau>' \<longrightarrow> (\<exists>v. n_s k = Some v \<and> type_of_val A v = Some (instantiate \<Omega> \<tau>'))"
   shows "\<forall>k \<tau>'.
             shift_env 1 0 \<Delta> k = Some \<tau>' \<longrightarrow> (\<exists>v. n_s k = Some v \<and> type_of_val A v = Some (instantiate (t # \<Omega>) \<tau>'))"
   oops
+*)
 
 lemma instantiate_shift: "wf_ty (length \<Omega>) \<tau> \<Longrightarrow> instantiate (t#\<Omega>) (shiftT 1 0 \<tau>) = instantiate \<Omega> \<tau>"
   by (induction \<tau>) (auto simp add: list_all_iff)
@@ -261,7 +263,7 @@ theorem progress:
   assumes
           Closed_\<Omega>:"list_all closed \<Omega>" and
           "\<forall> k \<tau>'. (\<Delta> k = Some \<tau>') \<longrightarrow> wf_ty (length \<Omega>) \<tau>'" and
-          "\<forall> k \<tau>'. (\<Delta> k = Some \<tau>') \<longrightarrow> (\<exists>v. (n_s k = Some v) \<and> type_of_val A v = Some (instantiate \<Omega> \<tau>'))" and
+          "\<forall> k \<tau>'. (\<Delta> k = Some \<tau>') \<longrightarrow> (\<exists>v. (n_s k = Some v) \<and> type_of_val A v = instantiate \<Omega> \<tau>')" and
           Wf_\<Gamma>:"fun_interp_wf A F \<Gamma>" and
           Wf_F:"list_all (wf_fdecl \<circ> snd) F"
   shows "F, \<Delta> \<turnstile> e : \<tau> \<Longrightarrow> expr_is_defined n_s e \<Longrightarrow>  wf_expr (length \<Omega>) e \<Longrightarrow>  \<exists>v. A,(F,\<Gamma>),\<Omega> \<turnstile> \<langle>e,n_s\<rangle> \<Down> v" and
@@ -279,7 +281,7 @@ next
 next
   case (TypUnOp uop arg_ty ret_ty \<Delta> e)
   from this obtain v' where RedE:"A,(F, \<Gamma>), \<Omega> \<turnstile> \<langle>e,n_s\<rangle> \<Down> v'" by fastforce
-  hence "type_of_val A v' = Some (TPrim arg_ty)" 
+  hence "type_of_val A v' = TPrim arg_ty" 
     using TypUnOp preservation(1)[OF \<open>list_all closed \<Omega>\<close> TypUnOp.prems(5) Wf_\<Gamma> Wf_F]
     by fastforce  
   thus ?case using \<open>unop_type uop = (arg_ty, ret_ty)\<close> unop_progress RedE RedUnOp
@@ -288,10 +290,10 @@ next
   case (TypBinOpMono bop left_ty right_ty ret_ty \<Delta> e1 e2)
   from this obtain v1 v2 where RedLeft:"A,(F, \<Gamma>),\<Omega> \<turnstile> \<langle>e1,n_s\<rangle> \<Down> v1" and  RedRight:"A,(F, \<Gamma>),\<Omega> \<turnstile> \<langle>e2,n_s\<rangle> \<Down> v2"
     by fastforce
-  moreover from RedLeft have "type_of_val A v1 = Some (TPrim left_ty)"
+  moreover from RedLeft have "type_of_val A v1 = TPrim left_ty"
     using TypBinOpMono.IH TypBinOpMono.prems preservation(1)[OF \<open>list_all closed \<Omega>\<close> TypBinOpMono.prems(5) Wf_\<Gamma> Wf_F]
     by fastforce
-  moreover from RedRight have "type_of_val A v2 = Some (TPrim right_ty)"
+  moreover from RedRight have "type_of_val A v2 = TPrim right_ty"
     using TypBinOpMono.IH TypBinOpMono.prems preservation(1)[OF \<open>list_all closed \<Omega>\<close> TypBinOpMono.prems(5) Wf_\<Gamma> Wf_F]
     by fastforce
   ultimately show ?case using \<open>binop_type bop = Some ((left_ty, right_ty), ret_ty)\<close> binop_progress RedBinOp
@@ -320,10 +322,10 @@ next
        FunSingleWf:"fun_interp_single_wf A (n_ty_params, args_ty, ret_ty) fi"
     using fun_interp_wf_def by blast 
   from RedArgs have 
-    "map (type_of_val A) vargs = map Some (map (instantiate \<Omega>) (map (msubstT_opt ty_params) args_ty))"
+    "map (type_of_val A) vargs = map (instantiate \<Omega>) (map (msubstT_opt ty_params) args_ty)"
     using preservation(2)[OF \<open>list_all closed \<Omega>\<close> TypFunExp.prems(5) Wf_\<Gamma> Wf_F] TypFunExp.prems TypFunExp.IH
     by (meson wf_expr.simps(5))
-  hence "map (type_of_val A) vargs = map Some (map (instantiate (map (instantiate \<Omega>) ty_params)) args_ty)"     
+  hence "map (type_of_val A) vargs = map (instantiate (map (instantiate \<Omega>) ty_params)) args_ty"     
     by (simp only: InstMSubst)
   moreover from \<open>length args = length args_ty\<close> and RedArgs have "length vargs = length args_ty"
     using red_exprs_length by fastforce
@@ -334,32 +336,32 @@ next
   with RedArgs show ?case by (metis Mem RedFunOp snd_conv)    
 next
   case (TypForall \<Delta> ty e)
-  have RedBody:"\<And>w. type_of_val A w = Some (instantiate \<Omega> ty) \<Longrightarrow> \<exists>v'. A, (F, \<Gamma>), \<Omega> \<turnstile> \<langle>e, ext_env n_s w\<rangle> \<Down> v'"
+  have RedBody:"\<And>w. type_of_val A w = instantiate \<Omega> ty \<Longrightarrow> \<exists>v'. A, (F, \<Gamma>), \<Omega> \<turnstile> \<langle>e, ext_env n_s w\<rangle> \<Down> v'"
     apply (rule TypForall.IH)
     using \<open>expr_is_defined n_s (Forall ty e)\<close> expr_is_defined.simps(6) apply blast
     using TypForall.prems by auto
-  have EnvCorres:"\<And>w. type_of_val A w = Some (instantiate \<Omega> ty) \<Longrightarrow> \<forall>k \<tau>'. (ext_env \<Delta> ty) k = Some \<tau>' \<longrightarrow> 
-                (\<exists>v. (ext_env n_s w) k = Some v \<and> type_of_val A v = Some (instantiate \<Omega> \<tau>'))"
+  have EnvCorres:"\<And>w. type_of_val A w = instantiate \<Omega> ty \<Longrightarrow> \<forall>k \<tau>'. (ext_env \<Delta> ty) k = Some \<tau>' \<longrightarrow> 
+                (\<exists>v. (ext_env n_s w) k = Some v \<and> type_of_val A v = instantiate \<Omega> \<tau>')"
     using TypForall.prems(5)
     by simp
   
-  have RedBodyTy:"\<And>w v'. type_of_val A w = Some (instantiate \<Omega> ty) \<Longrightarrow> A, (F, \<Gamma>), \<Omega> \<turnstile> \<langle>e, ext_env n_s w\<rangle> \<Down> v' \<Longrightarrow>
-        type_of_val A v' = Some (TPrim TBool)"
+  have RedBodyTy:"\<And>w v'. type_of_val A w = instantiate \<Omega> ty \<Longrightarrow> A, (F, \<Gamma>), \<Omega> \<turnstile> \<langle>e, ext_env n_s w\<rangle> \<Down> v' \<Longrightarrow>
+        type_of_val A v' = TPrim TBool"
     using preservation(1)[OF \<open>list_all closed \<Omega>\<close> EnvCorres Wf_\<Gamma> Wf_F]
           TypForall.IH(1) TypForall.prems(2)
     by (metis instantiate.simps(2) wf_expr.simps(6)) 
   show ?case
-  proof (cases "\<forall> w. type_of_val A w = Some (instantiate \<Omega> ty) \<longrightarrow> A, (F, \<Gamma>), \<Omega> \<turnstile> \<langle>e, ext_env n_s w\<rangle> \<Down> LitV (LBool True)")
+  proof (cases "\<forall> w. type_of_val A w = instantiate \<Omega> ty \<longrightarrow> A, (F, \<Gamma>), \<Omega> \<turnstile> \<langle>e, ext_env n_s w\<rangle> \<Down> LitV (LBool True)")
     case True
     show ?thesis
       using RedForAllTrue True by blast   
   next
     case False
     from this obtain w where
-       "type_of_val A w = Some (instantiate \<Omega> ty)" and "\<not> (A,(F, \<Gamma>),\<Omega> \<turnstile> \<langle>e, ext_env n_s w\<rangle> \<Down> LitV (LBool True))"
+       "type_of_val A w = instantiate \<Omega> ty" and "\<not> (A,(F, \<Gamma>),\<Omega> \<turnstile> \<langle>e, ext_env n_s w\<rangle> \<Down> LitV (LBool True))"
       by auto
     moreover from this RedBody RedBodyTy obtain w' where "A,(F, \<Gamma>),\<Omega> \<turnstile> \<langle>e, ext_env n_s w\<rangle> \<Down> w'"
-      and "type_of_val A w' = Some (TPrim (TBool))"
+      and "type_of_val A w' = TPrim (TBool)"
     by fastforce
     ultimately show ?thesis
       by (metis (full_types) RedForAllFalse type_of_val_bool_elim) 
@@ -367,31 +369,31 @@ next
 next
   case (TypExists \<Delta> ty e)
   (*  proof is almost identical to TypForall, TODO: re-use proof *)
-  have RedBody:"\<And>w. type_of_val A w = Some (instantiate \<Omega> ty) \<Longrightarrow> \<exists>v'. A, (F, \<Gamma>), \<Omega> \<turnstile> \<langle>e, ext_env n_s w\<rangle> \<Down> v'"
+  have RedBody:"\<And>w. type_of_val A w = instantiate \<Omega> ty \<Longrightarrow> \<exists>v'. A, (F, \<Gamma>), \<Omega> \<turnstile> \<langle>e, ext_env n_s w\<rangle> \<Down> v'"
     apply (rule TypExists.IH)
     using \<open>expr_is_defined n_s (Exists ty e)\<close> expr_is_defined.simps(7) apply blast
     using TypExists.prems by auto
-  have EnvCorres:"\<And>w. type_of_val A w = Some (instantiate \<Omega> ty) \<Longrightarrow> \<forall>k \<tau>'. (ext_env \<Delta> ty) k = Some \<tau>' \<longrightarrow> 
-        (\<exists>v. (ext_env n_s w) k = Some v \<and> type_of_val A v = Some (instantiate \<Omega> \<tau>'))"
+  have EnvCorres:"\<And>w. type_of_val A w = instantiate \<Omega> ty \<Longrightarrow> \<forall>k \<tau>'. (ext_env \<Delta> ty) k = Some \<tau>' \<longrightarrow> 
+        (\<exists>v. (ext_env n_s w) k = Some v \<and> type_of_val A v = instantiate \<Omega> \<tau>')"
     using TypExists.prems(5)
     by simp
   
-  have RedBodyTy:"\<And>w v'. type_of_val A w = Some (instantiate \<Omega> ty) \<Longrightarrow> A, (F, \<Gamma>), \<Omega> \<turnstile> \<langle>e, ext_env n_s w\<rangle> \<Down> v' \<Longrightarrow>
-        type_of_val A v' = Some (TPrim TBool)"
+  have RedBodyTy:"\<And>w v'. type_of_val A w = instantiate \<Omega> ty \<Longrightarrow> A, (F, \<Gamma>), \<Omega> \<turnstile> \<langle>e, ext_env n_s w\<rangle> \<Down> v' \<Longrightarrow>
+        type_of_val A v' = TPrim TBool"
     using preservation(1)[OF \<open>list_all closed \<Omega>\<close> EnvCorres Wf_\<Gamma> Wf_F]
           TypExists.IH(1) TypExists.prems(2) by (metis instantiate.simps(2) wf_expr.simps(7)) 
   show ?case
-  proof (cases "\<forall> w. type_of_val A w = Some (instantiate \<Omega> ty) \<longrightarrow> A, (F, \<Gamma>), \<Omega> \<turnstile> \<langle>e, ext_env n_s w\<rangle> \<Down> LitV (LBool False)")
+  proof (cases "\<forall> w. type_of_val A w = instantiate \<Omega> ty \<longrightarrow> A, (F, \<Gamma>), \<Omega> \<turnstile> \<langle>e, ext_env n_s w\<rangle> \<Down> LitV (LBool False)")
     case True
     show ?thesis
       using RedExistsFalse True by blast   
   next
     case False
     from this obtain w where
-       "type_of_val A w = Some (instantiate \<Omega> ty)" and "\<not> (A,(F, \<Gamma>),\<Omega> \<turnstile> \<langle>e, ext_env n_s w\<rangle> \<Down> LitV (LBool False))"
+       "type_of_val A w = instantiate \<Omega> ty" and "\<not> (A,(F, \<Gamma>),\<Omega> \<turnstile> \<langle>e, ext_env n_s w\<rangle> \<Down> LitV (LBool False))"
       by auto
     moreover from this RedBody RedBodyTy obtain w' where "A,(F, \<Gamma>),\<Omega> \<turnstile> \<langle>e, ext_env n_s w\<rangle> \<Down> w'"
-      and "type_of_val A w' = Some (TPrim (TBool))"
+      and "type_of_val A w' = TPrim (TBool)"
     by fastforce
     ultimately show ?thesis
       by (metis (full_types) RedExistsTrue type_of_val_bool_elim) 
@@ -409,7 +411,7 @@ next
   have Closed\<Omega>Ext: "\<And>t. closed t \<Longrightarrow> list_all closed (t#\<Omega>)"
     using \<open>list_all closed \<Omega>\<close> by simp
 
-  have RedBodyTy:"\<And>t v. closed t \<Longrightarrow> A,(F, \<Gamma>), t#\<Omega> \<turnstile> \<langle>e, n_s\<rangle> \<Down> v \<Longrightarrow> type_of_val A v = Some (instantiate (t#\<Omega>) (TPrim TBool))"
+  have RedBodyTy:"\<And>t v. closed t \<Longrightarrow> A,(F, \<Gamma>), t#\<Omega> \<turnstile> \<langle>e, n_s\<rangle> \<Down> v \<Longrightarrow> type_of_val A v = instantiate (t#\<Omega>) (TPrim TBool)"
     apply (rule preservation(1)[where ?\<Delta>="shift_env 1 0 \<Delta>" and ?n_s="n_s"])
           apply (simp add: \<open>list_all closed \<Omega>\<close>)
     using TypForallT.prems instantiate_shift
@@ -428,7 +430,7 @@ next
     case False
     from this obtain t where "closed t" and "\<not>(A,(F, \<Gamma>),t#\<Omega> \<turnstile> \<langle>e, n_s\<rangle> \<Down> LitV (LBool True))" by auto
     moreover from this RedBody RedBodyTy obtain w' where "A,(F, \<Gamma>),(t#\<Omega>) \<turnstile> \<langle>e, n_s\<rangle> \<Down> w'"
-      and "type_of_val A w' = Some (TPrim (TBool))" by fastforce
+      and "type_of_val A w' = TPrim (TBool)" by fastforce
     ultimately show ?thesis
       by (metis (full_types) RedForallT_False type_of_val_bool_elim)
   qed
@@ -447,7 +449,7 @@ next
   have Closed\<Omega>Ext: "\<And>t. closed t \<Longrightarrow> list_all closed (t#\<Omega>)"
     using \<open>list_all closed \<Omega>\<close> by simp
 
-  have RedBodyTy:"\<And>t v. closed t \<Longrightarrow> A,(F, \<Gamma>), t#\<Omega> \<turnstile> \<langle>e, n_s\<rangle> \<Down> v \<Longrightarrow> type_of_val A v = Some (instantiate (t#\<Omega>) (TPrim TBool))"
+  have RedBodyTy:"\<And>t v. closed t \<Longrightarrow> A,(F, \<Gamma>), t#\<Omega> \<turnstile> \<langle>e, n_s\<rangle> \<Down> v \<Longrightarrow> type_of_val A v = instantiate (t#\<Omega>) (TPrim TBool)"
     apply (rule preservation(1)[where ?\<Delta>="shift_env 1 0 \<Delta>" and ?n_s="n_s"])
           apply (simp add: \<open>list_all closed \<Omega>\<close>)
     using TypExistsT.prems instantiate_shift
@@ -456,8 +458,7 @@ next
        apply (rule Wf_F)
       apply (rule TypExistsT.IH(1))
     using TypExistsT.prems apply simp_all
-   done
-  
+    done  
   show ?case
   proof (cases "\<forall>t. closed t \<longrightarrow> A,(F, \<Gamma>),t#\<Omega> \<turnstile> \<langle>e, n_s\<rangle> \<Down> LitV (LBool False)")
     case True
@@ -467,7 +468,7 @@ next
     case False
     from this obtain t where "closed t" and "\<not>(A,(F, \<Gamma>),t#\<Omega> \<turnstile> \<langle>e, n_s\<rangle> \<Down> LitV (LBool False))" by auto
     moreover from this RedBody RedBodyTy obtain w' where "A,(F, \<Gamma>),(t#\<Omega>) \<turnstile> \<langle>e, n_s\<rangle> \<Down> w'"
-      and "type_of_val A w' = Some (TPrim (TBool))" by fastforce
+      and "type_of_val A w' = TPrim TBool" by fastforce
     ultimately show ?thesis
      by (metis (full_types) RedExistsT_True type_of_val_bool_elim)
   qed
